complete F* lib
(se prendre la tête pour pas grand chose)

Trees.fst
@@ -2,7 +2,6 @@ module Trees
 
 module M = FStar.Math.Lib
 
-#set-options "--fuel 10 --ifuel 10 --z3rlimit 20"
 
 (*** Type definitions *)
 
@@ -14,6 +13,10 @@ type tree (a: Type) =
 
 let csize (#a: Type) (t: tree a{Node? t}) =
   let Node _ _ _ s = t in s
+let cleft (#a: Type) (t: tree a{Node? t}) =
+  let Node _ l _ _ = t in l
+let cright (#a: Type) (t: tree a{Node? t}) =
+  let Node _ _ r _ = t in r
 
 (**** Binary search trees *)
 
@@ -50,7 +53,6 @@ let rec is_bst (#a: Type) (compare : cmp a) (x: tree a) : bool =
     forall_keys left (key_left compare data) &&
     forall_keys right (key_right compare data)
 
-let bst (a: Type) (cmp:cmp a) = x:tree a {is_bst cmp x}
 
 let rec size_of_tree (#a: Type) (x: tree a) : Tot nat (decreases x) =
   match x with
@@ -68,6 +70,8 @@ let rec is_wds (#a: Type) (x: tree a) : Tot (bool & nat) (decreases x) =
       b1 && b2 && size = s, s
 
 let wds (a: Type) = x:tree a {fst (is_wds x)}
+
+let bst (a: Type) (cmp:cmp a) = x:wds a {is_bst cmp x}
 
 let rec equiv_sot_wds (#a: Type) (x: tree a) :
   Lemma (let b, s = is_wds x in
@@ -102,8 +106,6 @@ let induction_wds (#a: Type) (x: a) (l r:wds a)
   equiv_sot_wds r;
   assert (fst (is_wds t));
   ()
-
-
 (*** Operations *)
 
 (**** Lookup *)
@@ -129,8 +131,10 @@ let rec height (#a: Type) (x: tree a) : nat =
   match x with
   | Leaf -> 0
   | Node data left right _ ->
-    if height left > height right then (height left) + 1
-    else (height right) + 1
+    let hleft = height left in
+    let hright = height right in
+    if hleft > hright then hleft + 1
+    else hright + 1
 
 (**** Append *)
 let aux_size_left_subtree (#a: Type) (t1: tree a) (t2: tree a)
@@ -218,18 +222,44 @@ let append_right (#a: Type) (t: wds a) (v: a)
 
 (**** BST insertion *)
 
-let rec insert_bst (#a: Type) (cmp:cmp a) (x: bst a cmp) (key: a) : tree a =
+let rec insert_bst_aux (#a: Type) (cmp:cmp a) (x: bst a cmp) (key: a)
+  : tree a =
   match x with
   | Leaf -> Node key Leaf Leaf 1
   | Node data left right size ->
     let delta = cmp data key in
     if delta >= 0 then begin
-      let new_left = insert_bst cmp left key in
+      let new_left = insert_bst_aux cmp left key in
       Node data new_left right (size + 1)
     end else begin
-      let new_right = insert_bst cmp right key in
+      let new_right = insert_bst_aux cmp right key in
       Node data left new_right (size + 1)
     end
+
+let rec insert_bst_aux_size (#a: Type) (cmp:cmp a) (x: bst a cmp) (key: a)
+  : Lemma (
+    size_of_tree (insert_bst_aux cmp x key) == size_of_tree x + 1 /\
+    fst (is_wds (insert_bst_aux cmp x key))
+  )
+  = match x with
+  | Leaf -> ()
+  | Node data left right size ->
+    let delta = cmp data key in
+    if delta >= 0 then begin
+      let new_left = insert_bst_aux cmp left key in
+      insert_bst_aux_size cmp left key;
+      aux_size_left_subtree left new_left;
+      induction_wds data new_left right
+    end else begin
+      let new_right = insert_bst_aux cmp right key in
+      insert_bst_aux_size cmp right key;
+      aux_size_right_subtree right (insert_bst_aux cmp right key);
+      induction_wds data left new_right
+    end
+
+let insert_bst (#a: Type) (cmp:cmp a) (x: bst a cmp) (key: a)
+  : wds a =
+  insert_bst_aux_size cmp x key; insert_bst_aux cmp x key
 
 let rec insert_bst_preserves_forall_keys
   (#a: Type)
@@ -279,10 +309,13 @@ let rec is_balanced (#a: Type) (x: tree a) : bool =
     is_balanced(right) &&
     is_balanced(left)
 
-let is_avl (#a: Type) (cmp:cmp a) (x: tree a) : prop =
+let is_avl (#a: Type) (cmp:cmp a) (x: wds a) : prop =
   is_bst cmp x /\ is_balanced x
 
-let avl (a: Type) (cmp:cmp a) = x: tree a {is_avl cmp x}
+let avl (a: Type) (cmp:cmp a) = x: wds a {is_avl cmp x}
+
+let get (#a: Type) (v: option a{Some? v}) : a =
+  let Some v' = v in v'
 
 let sot_wds (#a: Type) (r: wds a) : nat =
   match r with
@@ -303,19 +336,19 @@ t1   z   =>   x   t3
 
 let rotate_left (#a: Type) (r: tree a) : option (tree a) =
   match r with
-  | Node x t1 (Node z t2 t3 0) 0 -> Some (Node z (Node x t1 t2 0) t3 0)
+  | Node x t1 (Node z t2 t3 _) _ -> Some (Node z (Node x t1 t2 0) t3 0)
   | _ -> None
 
 let rotate_left_wds (#a: Type) (r: wds a) : option (wds a) =
   match r with
   | Node x t1 (Node z t2 t3 _) s ->
-      let sx = sot_wds t1 + sot_wds t2 + 1 in
-      let tx = Node x t1 t2 sx in
+      let s12 = sot_wds t1 + sot_wds t2 + 1 in
+      let t12 = Node x t1 t2 s12 in
       induction_wds x t1 t2;
-      assert (fst (is_wds tx));
-      let sz = sx + sot_wds t3 + 1 in
-      assert (sz == s);
-      Some (Node z (Node x t1 t2 sx) t3 s)
+      assert (fst (is_wds t12));
+      let s123 = s12 + sot_wds t3 + 1 in
+      assert (s123 == s);
+      Some (Node z t12 t3 s)
   | _ -> None
 
 (*
@@ -326,7 +359,8 @@ t1 t2          t2 t3
 
 let rotate_right (#a: Type) (r: tree a) : option (tree a) =
   match r with
-  | Node x (Node z t1 t2 0) t3 0 -> Some (Node z t1 (Node x t2 t3 0) 0)
+  | Node x (Node z t1 t2 _) t3 _ ->
+      Some (Node z t1 (Node x t2 t3 0) 0)
   | _ -> None
 
 let rotate_right_wds (#a: Type) (r: wds a) : option (wds a) =
@@ -350,7 +384,8 @@ t1     z    =>   x     z
 
 let rotate_right_left (#a: Type) (r: tree a) : option (tree a) =
   match r with
-  | Node x t1 (Node z (Node y t2 t3 0) t4 0) 0 -> Some (Node y (Node x t1 t2 0) (Node z t3 t4 0) 0)
+  | Node x t1 (Node z (Node y t2 t3 _) t4 _) _ ->
+      Some (Node y (Node x t1 t2 0) (Node z t3 t4 0) 0)
   | _ -> None
 
 let rotate_right_left_wds (#a: Type) (r: wds a) : option (wds a) =
@@ -379,7 +414,7 @@ t1   y         t1 t2 t3 t4
 
 let rotate_left_right (#a: Type) (r: tree a) : option (tree a) =
   match r with
-  | Node x (Node z t1 (Node y t2 t3 0) 0) t4 0  -> Some (Node y (Node z t1 t2 0) (Node x t3 t4 0) 0)
+  | Node x (Node z t1 (Node y t2 t3 _) _) t4 _  -> Some (Node y (Node z t1 t2 0) (Node x t3 t4 0) 0)
   | _ -> None
 
 let rotate_left_right_wds (#a: Type) (r: wds a) : option (wds a) =
@@ -398,17 +433,48 @@ let rotate_left_right_wds (#a: Type) (r: wds a) : option (wds a) =
       Some (Node y t12 t34 s)
   | _ -> None
 
+(*
+let rotate_left_size (#a: Type) (r: wds a)
+  : Lemma
+  (requires Some? (rotate_left_wds r))
+  (ensures size_of_tree (get (rotate_left_wds r)) == size_of_tree r)
+  = ()
+
+let rotate_right_size (#a: Type) (r: wds a)
+  : Lemma
+  (requires Some? (rotate_right_wds r))
+  (ensures size_of_tree (get (rotate_right_wds r)) == size_of_tree r)
+  = ()
+
+let rotate_right_left_size (#a: Type) (r: wds a)
+  : Lemma
+  (requires Some? (rotate_right_left_wds r))
+  (ensures
+  size_of_tree (get (rotate_right_left_wds r)) == size_of_tree r)
+  = ()
+
+let rotate_left_right_size (#a: Type) (r: wds a)
+  : Lemma
+  (requires Some? (rotate_right_left_wds r))
+  (ensures
+  size_of_tree (get (rotate_right_left_wds r)) == size_of_tree r)
+  = ()
+*)
+
 (** rotate preserves bst *)
 let rec forall_keys_trans (#a: Type) (t: tree a) (cond1 cond2: a -> bool)
-  : Lemma (requires (forall x. cond1 x ==> cond2 x) /\ forall_keys t cond1)
-          (ensures forall_keys t cond2)
+  : Lemma
+  (requires (forall x. cond1 x ==> cond2 x) /\ forall_keys t cond1)
+  (ensures forall_keys t cond2)
   = match t with
   | Leaf -> ()
   | Node data left right _ ->
     forall_keys_trans left cond1 cond2; forall_keys_trans right cond1 cond2
 
 let rotate_left_bst (#a:Type) (cmp:cmp a) (r:wds a)
-  : Lemma (requires is_bst cmp r /\ Some? (rotate_left r)) (ensures is_bst cmp (Some?.v (rotate_left r)))
+  : Lemma
+  (requires is_bst cmp r /\ Some? (rotate_left_wds r))
+  (ensures is_bst cmp (Some?.v (rotate_left_wds r)))
   = match r with
   | Node x t1 (Node z t2 t3 s23) _ ->
       assert (is_bst cmp (Node z t2 t3 s23));
@@ -417,7 +483,9 @@ let rotate_left_bst (#a:Type) (cmp:cmp a) (r:wds a)
       forall_keys_trans t1 (key_left cmp x) (key_left cmp z)
 
 let rotate_right_bst (#a:Type) (cmp:cmp a) (r:wds a)
-  : Lemma (requires is_bst cmp r /\ Some? (rotate_right r)) (ensures is_bst cmp (Some?.v (rotate_right r)))
+  : Lemma
+  (requires is_bst cmp r /\ Some? (rotate_right_wds r))
+  (ensures is_bst cmp (Some?.v (rotate_right_wds r)))
   = match r with
   | Node x (Node z t1 t2 s12) t3 _ ->
       assert (is_bst cmp (Node z t1 t2 s12));
@@ -426,7 +494,9 @@ let rotate_right_bst (#a:Type) (cmp:cmp a) (r:wds a)
       forall_keys_trans t3 (key_right cmp x) (key_right cmp z)
 
 let rotate_right_left_bst (#a:Type) (cmp:cmp a) (r:wds a)
-  : Lemma (requires is_bst cmp r /\ Some? (rotate_right_left r)) (ensures is_bst cmp (Some?.v (rotate_right_left r)))
+  : Lemma
+  (requires is_bst cmp r /\ Some? (rotate_right_left_wds r))
+  (ensures is_bst cmp (Some?.v (rotate_right_left_wds r)))
   = match r with
   | Node x t1 (Node z (Node y t2 t3 s23) t4 s234) _ ->
     // Node y (Node x t1 t2) (Node z t3 t4)
@@ -449,9 +519,10 @@ let rotate_right_left_bst (#a:Type) (cmp:cmp a) (r:wds a)
     forall_keys_trans t4 (key_right cmp z) (key_right cmp y);
     assert (forall_keys right (key_right cmp y))
 
-
 let rotate_left_right_bst (#a:Type) (cmp:cmp a) (r:wds a)
-  : Lemma (requires is_bst cmp r /\ Some? (rotate_left_right r)) (ensures is_bst cmp (Some?.v (rotate_left_right r)))
+  : Lemma
+  (requires is_bst cmp r /\ Some? (rotate_left_right_wds r))
+  (ensures is_bst cmp (Some?.v (rotate_left_right_wds r)))
   = match r with
   | Node x (Node z t1 (Node y t2 t3 s23) s123) t4 _ ->
     // Node y (Node z t1 t2) (Node x t3 t4)
@@ -477,8 +548,9 @@ let rotate_left_right_bst (#a:Type) (cmp:cmp a) (r:wds a)
 (** Same elements before and after rotate **)
 
 let rotate_left_key_left (#a:Type) (cmp:cmp a) (r:wds a) (root:a)
-  : Lemma (requires forall_keys r (key_left cmp root) /\ Some? (rotate_left r))
-          (ensures  forall_keys (Some?.v (rotate_left r)) (key_left cmp root))
+  : Lemma
+  (requires forall_keys r (key_left cmp root) /\ Some? (rotate_left r))
+  (ensures  forall_keys (Some?.v (rotate_left r)) (key_left cmp root))
   = match r with
   | Node x t1 (Node z t2 t3 s23) _ ->
       let s12 = sot_wds t1 + sot_wds t2 + 1 in
@@ -486,8 +558,9 @@ let rotate_left_key_left (#a:Type) (cmp:cmp a) (r:wds a) (root:a)
       assert (forall_keys (Node x t1 t2 s12) (key_left cmp root))
 
 let rotate_left_key_right (#a:Type) (cmp:cmp a) (r:wds a) (root:a)
-  : Lemma (requires forall_keys r (key_right cmp root) /\ Some? (rotate_left r))
-          (ensures  forall_keys (Some?.v (rotate_left r)) (key_right cmp root))
+  : Lemma
+  (requires forall_keys r (key_right cmp root) /\ Some? (rotate_left r))
+  (ensures  forall_keys (Some?.v (rotate_left r)) (key_right cmp root))
   = match r with
   | Node x t1 (Node z t2 t3 s23) _ ->
       let s12 = sot_wds t1 + sot_wds t2 + 1 in
@@ -495,8 +568,9 @@ let rotate_left_key_right (#a:Type) (cmp:cmp a) (r:wds a) (root:a)
       assert (forall_keys (Node x t1 t2 s12) (key_right cmp root))
 
 let rotate_right_key_left (#a:Type) (cmp:cmp a) (r:wds a) (root:a)
-  : Lemma (requires forall_keys r (key_left cmp root) /\ Some? (rotate_right r))
-          (ensures  forall_keys (Some?.v (rotate_right r)) (key_left cmp root))
+  : Lemma
+  (requires forall_keys r (key_left cmp root) /\ Some? (rotate_right r))
+  (ensures  forall_keys (Some?.v (rotate_right r)) (key_left cmp root))
   = match r with
   | Node x (Node z t1 t2 s12) t3 _ ->
       let s23 = sot_wds t2 + sot_wds t3 + 1 in
@@ -504,8 +578,9 @@ let rotate_right_key_left (#a:Type) (cmp:cmp a) (r:wds a) (root:a)
       assert (forall_keys (Node x t2 t3 s23) (key_left cmp root))
 
 let rotate_right_key_right (#a:Type) (cmp:cmp a) (r:wds a) (root:a)
-  : Lemma (requires forall_keys r (key_right cmp root) /\ Some? (rotate_right r))
-          (ensures  forall_keys (Some?.v (rotate_right r)) (key_right cmp root))
+  : Lemma
+  (requires forall_keys r (key_right cmp root) /\ Some? (rotate_right r))
+  (ensures  forall_keys (Some?.v (rotate_right r)) (key_right cmp root))
   = match r with
   | Node x (Node z t1 t2 s12) t3 _ ->
       let s23 = sot_wds t2 + sot_wds t3 + 1 in
@@ -513,8 +588,9 @@ let rotate_right_key_right (#a:Type) (cmp:cmp a) (r:wds a) (root:a)
       assert (forall_keys (Node x t2 t3 s23) (key_right cmp root))
 
 let rotate_right_left_key_left (#a:Type) (cmp:cmp a) (r:wds a) (root:a)
-  : Lemma (requires forall_keys r (key_left cmp root) /\ Some? (rotate_right_left r))
-          (ensures  forall_keys (Some?.v (rotate_right_left r)) (key_left cmp root))
+  : Lemma
+  (requires forall_keys r (key_left cmp root) /\ Some? (rotate_right_left r))
+  (ensures  forall_keys (Some?.v (rotate_right_left r)) (key_left cmp root))
   = match r with
   | Node x t1 (Node z (Node y t2 t3 s23) t4 s234) _ ->
     assert (forall_keys (Node z (Node y t2 t3 s23) t4 s234) (key_left cmp root));
@@ -527,8 +603,9 @@ let rotate_right_left_key_left (#a:Type) (cmp:cmp a) (r:wds a) (root:a)
     assert (forall_keys right (key_left cmp root))
 
 let rotate_right_left_key_right (#a:Type) (cmp:cmp a) (r:wds a) (root:a)
-  : Lemma (requires forall_keys r (key_right cmp root) /\ Some? (rotate_right_left r))
-          (ensures  forall_keys (Some?.v (rotate_right_left r)) (key_right cmp root))
+  : Lemma
+  (requires forall_keys r (key_right cmp root) /\ Some? (rotate_right_left r))
+  (ensures  forall_keys (Some?.v (rotate_right_left r)) (key_right cmp root))
   = match r with
   | Node x t1 (Node z (Node y t2 t3 s23) t4 s234) _ ->
     assert (forall_keys (Node z (Node y t2 t3 s23) t4 s234) (key_right cmp root));
@@ -541,8 +618,9 @@ let rotate_right_left_key_right (#a:Type) (cmp:cmp a) (r:wds a) (root:a)
     assert (forall_keys right (key_right cmp root))
 
 let rotate_left_right_key_left (#a:Type) (cmp:cmp a) (r:wds a) (root:a)
-  : Lemma (requires forall_keys r (key_left cmp root) /\ Some? (rotate_left_right r))
-          (ensures  forall_keys (Some?.v (rotate_left_right r)) (key_left cmp root))
+  : Lemma
+  (requires forall_keys r (key_left cmp root) /\ Some? (rotate_left_right r))
+  (ensures  forall_keys (Some?.v (rotate_left_right r)) (key_left cmp root))
   = match r with
   | Node x (Node z t1 (Node y t2 t3 s23) s123) t4 _ ->
     assert (forall_keys (Node z t1 (Node y t2 t3 s23) s123) (key_left cmp root));
@@ -555,8 +633,9 @@ let rotate_left_right_key_left (#a:Type) (cmp:cmp a) (r:wds a) (root:a)
     assert (forall_keys right (key_left cmp root))
 
 let rotate_left_right_key_right (#a:Type) (cmp:cmp a) (r:wds a) (root:a)
-  : Lemma (requires forall_keys r (key_right cmp root) /\ Some? (rotate_left_right r))
-          (ensures  forall_keys (Some?.v (rotate_left_right r)) (key_right cmp root))
+  : Lemma
+  (requires forall_keys r (key_right cmp root) /\ Some? (rotate_left_right r))
+  (ensures  forall_keys (Some?.v (rotate_left_right r)) (key_right cmp root))
   = match r with
   | Node x (Node z t1 (Node y t2 t3 s23) s123) t4 _ ->
     assert (forall_keys (Node z t1 (Node y t2 t3 s23) s123) (key_right cmp root));
@@ -570,17 +649,15 @@ let rotate_left_right_key_right (#a:Type) (cmp:cmp a) (r:wds a) (root:a)
 
 
 (** Balancing operation for AVLs *)
-(*)
+
 let rebalance_avl (#a: Type) (x: tree a) : tree a =
     match x with
     | Leaf -> x
-    | Node data left right ->
-
+    | Node data left right _ ->
       if is_balanced x then x
       else (
-
         if height left - height right > 1 then (
-          let Node ldata lleft lright = left in
+          let Node ldata lleft lright _ = left in
           if height lright > height lleft then (
             match rotate_left_right x with
             | Some y -> y
@@ -592,7 +669,7 @@ let rebalance_avl (#a: Type) (x: tree a) : tree a =
           )
 
         ) else if height left - height right < -1 then (
-          let Node rdata rleft rright = right in
+          let Node rdata rleft rright _ = right in
             if height rleft > height rright then (
               match rotate_right_left x with
               | Some y -> y
@@ -608,135 +685,180 @@ let rebalance_avl (#a: Type) (x: tree a) : tree a =
       )
 
 
-let rebalance_avl_proof (#a: Type) (cmp:cmp a) (x: tree a)
-  (root:a)
-  : Lemma
-  (requires is_bst cmp x /\ (
-    match x with
-    | Leaf -> True
-    | Node data left right ->
-      is_balanced left /\ is_balanced right /\
-      height left - height right <= 2 /\
-      height right - height left <= 2
+(*
+some changes with respect to previous version, as
+this function is intended to be only used after
+adding an element to a previously balanced tree:
+no need to go through this entire tree
+TODO : height as metadata to be retrieved in O(1)
+TODO : specify rotate_* as inline functions in C (benchmark the difference !)
+TODO : optimize rotate_*, remove matching and add precondition
+TODO : option.get
+*)
+
+let rebalance_avl_wds (#a: Type) (t: wds a) : wds a =
+  if Leaf? t then t else
+  let Node data left right size = t in
+  if height left - height right > 1 then (
+    let Node ldata lleft lright lsize = left in
+    if height lleft >= height lright then (
+      let r = rotate_right_wds t in
+      assert (Some? r);
+      get r
+    ) else (
+      let r = rotate_left_right_wds t in
+      assert (Some? r);
+      get r
     )
+  ) else if height right - height left > 1 then (
+    let Node rdata rleft rright rsize = right in
+    if height rleft > height rright then (
+      let r = rotate_right_left_wds t in
+      assert (Some? r);
+      get r
+    ) else (
+      let r = rotate_left_wds t in
+      assert (Some? r);
+      get r
+    )
+  ) else (
+    t
   )
-  (ensures is_avl cmp (rebalance_avl x) /\
-     (forall_keys x (key_left cmp root) ==> forall_keys (rebalance_avl x) (key_left cmp root)) /\
-     (forall_keys x (key_right cmp root) ==> forall_keys (rebalance_avl x) (key_right cmp root))
+
+let rebalance_avl_wds_size (#a: Type) (t: wds a)
+  : Lemma (size_of_tree (rebalance_avl_wds t) == size_of_tree t)
+  = ()
+
+#push-options "--fuel 2 --ifuel 2 --z3rlimit 20"
+
+let rebalance_avl_wds_proof (#a: Type) (cmp: cmp a) (t: wds a)
+  (root: a)
+  : Lemma
+  (requires is_bst cmp t /\ (
+    match t with
+    | Leaf -> True
+    | Node data left right _ ->
+        is_balanced left /\
+        is_balanced right /\
+        height left - height right <= 2 /\
+        height right - height left <= 2
+  ))
+  (ensures
+    is_avl cmp (rebalance_avl_wds t)
+    /\
+    (forall_keys t (key_left cmp root)
+      ==> forall_keys (rebalance_avl_wds t) (key_left cmp root)) /\
+    (forall_keys t (key_right cmp root)
+      ==> forall_keys (rebalance_avl_wds t) (key_right cmp root))
   )
   =
-    match x with
-    | Leaf -> ()
-    | Node data left right ->
-      let x_f = rebalance_avl x in
-      let Node f_data f_left f_right = x_f in
-      if is_balanced x then ()
-      else (
-        if height left - height right > 1 then (
-          assert (height left = height right + 2);
-          let Node ldata lleft lright = left in
-          if height lright > height lleft then (
-            assert (height left = height lright + 1);
-            rotate_left_right_bst cmp x;
-            Classical.move_requires (rotate_left_right_key_left cmp x) root;
-            Classical.move_requires (rotate_left_right_key_right cmp x) root;
+  if Leaf? t then () else
+  let Node _ left right _ = t in
+  if height left - height right > 1 then (
+    assert (height left - height right == 2);
+    let Node _ lleft lright _ = left in
+    if height lleft >= height lright then (
+      let r = rotate_right_wds t in
+      assert (Some? r);
+      let t' = get r in
+      rotate_right_bst cmp t;
+      Classical.move_requires (rotate_right_key_left cmp t) root;
+      Classical.move_requires (rotate_right_key_right cmp t) root;
+      assert (is_avl cmp t')
+    ) else (
+      let r = rotate_left_right_wds t in
+      assert (Some? r);
+      let t' = get r in
+      rotate_left_right_bst cmp t;
+      Classical.move_requires (rotate_left_right_key_left cmp t) root;
+      Classical.move_requires (rotate_left_right_key_right cmp t) root;
+      assert (is_avl cmp t')
+    )
+  ) else if height right - height left > 1 then (
+    assert (height right - height left == 2);
+    let Node _ rleft rright _ = right in
+    assert (is_balanced right);
+    if height rright >= height rleft then (
+      let r = rotate_left_wds t in
+      assert (Some? r);
+      let t' = get r in
+      rotate_left_bst cmp t;
+      Classical.move_requires (rotate_left_key_left cmp t) root;
+      Classical.move_requires (rotate_left_key_right cmp t) root;
+      assert (is_avl cmp t')
+    ) else (
+      let r = rotate_right_left_wds t in
+      assert (Some? r);
+      let t' = get r in
+      rotate_right_left_bst cmp t;
+      Classical.move_requires (rotate_right_left_key_left cmp t) root;
+      Classical.move_requires (rotate_right_left_key_right cmp t) root;
+      assert (is_avl cmp t')
+    )
+)
 
-            let Node y t2 t3 = lright in
-            let Node x (Node z t1 (Node y t2 t3)) t4 = x in
-            assert (f_data == y);
-            assert (f_left == Node z t1 t2);
-            assert (f_right == Node x t3 t4);
-            assert (lright == Node y t2 t3);
-
-            // Left part
-
-            assert (is_balanced lright);
-            assert (height t1 - height t2 <= 1);
-
-            assert (height t2 - height t1 <= 1);
-
-            assert (is_balanced t1);
-
-            assert (is_balanced (Node y t2 t3));
-            assert (is_balanced t2);
-
-            assert (is_balanced f_left);
-
-
-            // Right part
-            assert (height t3 - height t4 <= 1);
-            assert (height t4 - height t3 <= 1);
-
-            assert (is_balanced t3);
-            assert (is_balanced t4);
-            assert (is_balanced f_right)
-
-          ) else (
-            rotate_right_bst cmp x;
-            Classical.move_requires (rotate_right_key_left cmp x) root;
-            Classical.move_requires (rotate_right_key_right cmp x) root;
-
-            assert (is_balanced f_left);
-            assert (is_balanced f_right);
-            assert (is_balanced x_f)
-          )
-
-        ) else if height left - height right < -1 then (
-          let Node rdata rleft rright = right in
-          if height rleft > height rright then (
-            rotate_right_left_bst cmp x;
-            Classical.move_requires (rotate_right_left_key_left cmp x) root;
-            Classical.move_requires (rotate_right_left_key_right cmp x) root;
-
-            let Node x t1 (Node z (Node y t2 t3) t4) = x in
-            assert (f_data == y);
-            assert (f_left == Node x t1 t2);
-            assert (f_right == Node z t3 t4);
-
-            // Right part
-            assert (is_balanced rleft);
-            assert (height t3 - height t4 <= 1);
-            assert (height t4 - height t4 <= 1);
-
-            assert (is_balanced (Node y t2 t3));
-            assert (is_balanced f_right);
-
-            // Left part
-            assert (is_balanced t1);
-            assert (is_balanced t2);
-            assert (is_balanced f_left)
-
-          ) else (
-            rotate_left_bst cmp x;
-            Classical.move_requires (rotate_left_key_left cmp x) root;
-            Classical.move_requires (rotate_left_key_right cmp x) root;
-
-            assert (is_balanced f_left);
-            assert (is_balanced f_right);
-            assert (is_balanced x_f)
-          )
-        )
-      )
-
+#pop-options
 (** Insertion **)
 
-let rec insert_avl (#a: Type) (cmp:cmp a) (x: tree a) (key: a) : tree a =
+let rec insert_avl (#a: Type) (cmp:cmp a) (x: avl a cmp) (key: a)
+  : t:wds a{size_of_tree t == size_of_tree x + 1}
+  =
   match x with
-  | Leaf -> Node key Leaf Leaf
-  | Node data left right ->
+  | Leaf -> Node key Leaf Leaf 1
+  | Node data left right size ->
     let delta = cmp data key in
     if delta >= 0 then (
       let new_left = insert_avl cmp left key in
-      let tmp = Node data new_left right in
-      rebalance_avl tmp
+      let tmp = Node data new_left right (size + 1) in
+      //aux_size_left_subtree left new_left;
+      check x;
+      induction_wds data new_left right;
+      let t = rebalance_avl_wds tmp in
+      rebalance_avl_wds_size tmp;
+      t
     ) else (
       let new_right = insert_avl cmp right key in
-      let tmp = Node data left new_right in
-      rebalance_avl tmp
+      let tmp = Node data left new_right (size + 1) in
+      //aux_size_right_subtree right new_right;
+      check x;
+      induction_wds data left new_right;
+      let t = rebalance_avl_wds tmp in
+      rebalance_avl_wds_size tmp;
+      t
     )
 
-#push-options "--z3rlimit 50"
+(*
+let rec insert_avl_aux_height (#a: Type)
+  (cmp: cmp a) (x: avl a cmp) (key: a)
+  : Lemma (
+    height x <= height (insert_avl cmp x key) /\
+    height (insert_avl cmp x key) <= height x + 1
+  )
+  = match x with
+  | Leaf -> ()
+  | Node data left right size ->
+      let delta = cmp data key in
+      if delta >= 0 then
+        insert_avl_aux_height cmp left key
+      else
+        insert_avl_aux_height cmp right key
 
+let insert_avl_aux_height2 (#a: Type)
+  (cmp: cmp a) (x: avl a cmp) (key: a)
+  : Lemma
+  (
+    Node? x ==> (
+    let x2 = snd (insert_avl_aux cmp x key) in
+    height (cleft x) == height (cleft x2)
+    \/
+    height (cright x) == height (cright x2)
+  ))
+  = match x with
+  | Leaf -> ()
+  | Node data left right size -> ()
+*)
+
+#push-options "--fuel 1 --ifuel 1 --z3rlimit 50"
 let rec insert_avl_proof_aux (#a: Type) (cmp:cmp a) (x: avl a cmp) (key: a)
   (root:a)
 
@@ -748,35 +870,33 @@ let rec insert_avl_proof_aux (#a: Type) (cmp:cmp a) (x: avl a cmp) (key: a)
       height res <= height x + 1 /\
       (forall_keys x (key_left cmp root) /\ key_left cmp root key ==> forall_keys res (key_left cmp root)) /\
       (forall_keys x (key_right cmp root) /\ key_right cmp root key ==> forall_keys res (key_right cmp root)))
-
     )
   = match x with
   | Leaf -> ()
-  | Node data left right ->
+  | Node data left right size ->
     let delta = cmp data key in
     if delta >= 0 then (
       let new_left = insert_avl cmp left key in
-      let tmp = Node data new_left right in
+      let tmp = Node data new_left right (size+1) in
 
       insert_avl_proof_aux cmp left key data;
-      // Need this one for propagating that all elements are smaller than root
       insert_avl_proof_aux cmp left key root;
-
-      rebalance_avl_proof cmp tmp root
+      rebalance_avl_wds_proof cmp tmp root
 
     ) else (
       let new_right = insert_avl cmp right key in
-      let tmp = Node data left new_right in
+      let tmp = Node data left new_right (size+1) in
 
       insert_avl_proof_aux cmp right key data;
       insert_avl_proof_aux cmp right key root;
-
-      rebalance_avl_proof cmp tmp root
+      rebalance_avl_wds_proof cmp tmp root
     )
-
 #pop-options
 
 let insert_avl_proof (#a: Type) (cmp:cmp a) (x: avl a cmp) (key: a)
   : Lemma (requires is_avl cmp x) (ensures is_avl cmp (insert_avl cmp x key))
-  = Classical.forall_intro (Classical.move_requires (insert_avl_proof_aux cmp x key))
-*)
+  = Classical.forall_intro (
+      Classical.move_requires (
+        insert_avl_proof_aux cmp x key
+      )
+    )
